WIP connected components

dataplane/Examples/Label_Propagation_op.thy
@@ -14,7 +14,8 @@ fun unions_with where
 
 primrec list_span where
   \<open>list_span _ [] = ([], [])\<close>
-| \<open>list_span P (x # xs) = (if P x then let (ys, zs) = list_span P xs in (x # ys, zs) else ([], x # xs))\<close>
+| \<open>list_span P (x # xs) =
+    (if P x then let (ys, zs) = list_span P xs in (x # ys, zs) else ([], x # xs))\<close>
 
 lemma list_span_length_le:
   \<open>(ys, zs) = list_span P xs \<Longrightarrow> length ys \<le> length xs\<close>
@@ -43,8 +44,10 @@ lemma sorted_insort_union:
   \<open>sorted ys \<Longrightarrow> sorted (insort_union xs ys)\<close>
   by (induction xs) (simp_all add: insort_union_def fold_invariant sorted_insort_insert)
 
-record ('d, 'v :: linorder, 't1, 't2) label_propagation_state = \<open>(2, 'd, 'v \<times> 'v, 'v list list, ('t1, 't2) myprod) operator_state_ty2\<close> +
-  timestamps :: \<open>'t1 list\<close> graph :: \<open>'t1 \<Rightarrow> 'v \<Rightarrow> 'v list\<close> vertices :: \<open>'t1 \<Rightarrow> 'v list\<close> label :: \<open>'t1 \<Rightarrow> 'v \<Rightarrow> 'v\<close>
+record ('d, 'v :: linorder, 't1, 't2) label_propagation_state =
+  \<open>(2, 'd, 'v \<times> 'v, 'v set set, ('t1, 't2) myprod) operator_state_ty2\<close> +
+  timestamps :: \<open>'t1 list\<close> graph :: \<open>'t1 \<Rightarrow> 'v \<Rightarrow> 'v list\<close> vertices :: \<open>'t1 \<Rightarrow> 'v list\<close>
+  label :: \<open>'t1 \<Rightarrow> 'v \<Rightarrow> 'v\<close>
 
 definition neighbors where
   \<open>neighbors os t = (let ts = filter ((\<ge>) t) (timestamps os) in
@@ -54,12 +57,16 @@ definition all_vertices where
   \<open>all_vertices os t = (let ts = filter ((\<ge>) t) (timestamps os) in
   if is_Nil ts then vertices os t else mergesort_remdups (concat (map (vertices os) ts)))\<close>
 
+definition all_edges where
+  \<open>all_edges os t = {(v, w). w \<in> set (neighbors os t v)}\<close>
+
 definition min_label where
   \<open>min_label os t v = (let ts = filter ((\<ge>) t) (timestamps os) in
   if is_Nil ts then label os t v else Min (set (map (\<lambda>t. label os t v) ts)))\<close>
 
 (* Note: I assume that the timestamps of data read on port 0 are of the form "MyPair t1 0", i.e.,
 the second component is assumed to be always 0. *)
+(* Should the logic return a set of sets for the connected components or a list of lists? *)
 definition label_propagation_op_logic where
   \<open>label_propagation_op_logic os = cUn (cUn
   (case input os 0 of
@@ -70,7 +77,8 @@ definition label_propagation_op_logic where
         (l1, l2) = pairself (min_label os t1) (v1, v2);
         (v, l) = if l1 > l2 then (v1, l2) else (v2, l1);
         os' = os\<lparr>input := (input os)(0 := xs), timestamps := List.insert t1 (timestamps os),
-  graph := (graph os)(t1 := (graph os t1)(v1 := List.insert v2 (graph os t1 v1), v2 := List.insert v1 (graph os t1 v2))),
+  graph := (graph os)(t1 := (graph os t1)(v1 := List.insert v2 (graph os t1 v1),
+    v2 := List.insert v1 (graph os t1 v2))),
   vertices := (vertices os)(t1 := List.union [v1, v2] (vertices os t1)),
   label := (label os)(t1 := (label os t1)(v := l))\<rparr>;
         vs = neighbors os' t1 v;
@@ -83,18 +91,24 @@ definition label_propagation_op_logic where
   | (d, t) # xs \<Rightarrow>
     let (v, l) = de1 os d;
         t1 = myfst t;
-        os' = os\<lparr>input := (input os)(1 := xs), label := (label os)(t1 := (label os t1)(v := min (min_label os t1 v) l))\<rparr>;
+        os' = os\<lparr>input := (input os)(1 := xs),
+          label := (label os)(t1 := (label os t1)(v := min (min_label os t1 v) l))\<rparr>;
         vs = neighbors os t1 v;
         batch = if min_label os t1 v > l
           then map (\<lambda>v'. (en1 os (v', l), Cap t 1)) (filter (\<lambda>v'. min_label os t1 v' > l) vs)
           else []
     in {|drop_cap (produces os' batch) (Cap t 1)|}))
-  (let P = \<lambda>t. \<forall>n < length (all_vertices os (myfst t)). \<not> frontier_less_equal (front os 0 + front os 1) (MyPair (myfst t) n);
+  (let P = \<lambda>t. \<forall>n < length (all_vertices os (myfst t)).
+         \<not> frontier_less_equal (front os 0 + front os 1) (MyPair (myfst t) n);
        below_times = filter P (ocaps os 0);
        output_times = mergesort_remdups (map myfst below_times);
-       batch = map (\<lambda>t. let cap = Cap (MyPair t 0) 0 in
-        (en2 os (group_by (\<lambda>v1 v2. min_label os t v1 = min_label os t v2) (all_vertices os t)), cap)) output_times
-   in if batch = [] then {||} else {|drop_caps (produces os batch) (map (\<lambda>t. Cap t 0) below_times @ map (\<lambda>t. Cap t 1) (filter P (ocaps os 1)))|})\<close>
+       batch = map (\<lambda>t. let cap = Cap (MyPair t 0) 0 in (en2 os (set (map set
+          (group_by (\<lambda>v1 v2. min_label os t v1 = min_label os t v2) (all_vertices os t)))), cap))
+        output_times
+   in if batch = []
+        then {||}
+        else {|drop_caps (produces os batch) (map (\<lambda>t. Cap t 0) below_times
+          @ map (\<lambda>t. Cap t 1) (filter P (ocaps os 1)))|})\<close>
 
 definition label_propagation_op where
   \<open>label_propagation_op os = builder_op True cUNIV cUNIV os label_propagation_op_logic\<close>
